TFTP_Core.v
@@ -1,4 +1,5 @@
 Require Import ZArith.
+Require Import Coq.Strings.String.
 Require Import ZArith.BinInt.
 Require Import Ascii.
 Require Import List.
@@ -14,11 +15,9 @@ Local Open Scope char_scope.
 Axiom newline : ascii.
 Definition hello := ["h"; "i"].
 
-Inductive maybe (t : Set) := just : t -> maybe t | nothing : maybe t. 
-
-Definition message : Set := list ascii.
+Definition message : Set := string.
 Inductive transfer : Set := upload : message -> transfer | download : message -> transfer.
-Inductive action : Set := send : message -> N -> action | continue : action | terminate : action.
+Inductive action : Set := send : message -> N -> action | terminate : action.
 
 Inductive protocol_state : Set
  := waiting_for_init_ack
@@ -28,43 +27,56 @@ Inductive protocol_state : Set
 
 Record state : Set := mkState
  { fsm : protocol_state
- ; previousMessage : maybe message
+ ; previousMessage : option message
  ; mytid : N
+ ; actions : list action
  }.
 Inductive input_event : Set := incoming : message -> N -> input_event | timeout : input_event.
 
-(* Monadic code inspired by  file:///home/radeusgd/Projekty/TFTP/reference/MemMonad.html  TODO true link*)
-Definition stateM (ret : Set) := state -> state * ret.
+(* Monadic code inspired by  http://adam.chlipala.net/poplmark/compile/coqdoc/MemMonad.html *)
+Definition serverM (ret : Set) := state -> state * option ret.
+(* TODO thinking about including an action writer in the used Monad to have multiple possible actions + error semantics (fail action) *)
 
-Definition SReturn (T : Set) (v : T) : stateM T :=
-  fun m => (m, v).
+Definition Return (T : Set) (v : T) : serverM T :=
+  fun m => (m, Some v).
 
 (*  operations on state *)
-Definition GetFSM : stateM protocol_state :=
-  fun m => (m, fsm m).
+Definition GetFSM : serverM protocol_state :=
+  fun m => (m, Some (fsm m)).
 
-Definition SetFSM (s : protocol_state) : stateM unit :=
-  fun m => (mkState s (previousMessage m) (mytid m), tt).
+Definition SetFSM (s : protocol_state) : serverM unit :=
+  fun m => (mkState s (previousMessage m) (mytid m) (actions m), Some tt).
 
-Definition SBind (T1 T2 : Set) (M1 : stateM T1) (M2 : T1 -> stateM T2) : stateM T2 :=
+Definition DoAction (a : action) : serverM unit :=
+  fun m => (mkState (fsm m) (previousMessage m) (mytid m) (a :: actions m), Some tt).
+
+Definition Send (msg : message) (to : N) : serverM unit :=
+  DoAction (send msg to).
+
+Definition Fail (T : Set) : serverM T := fun m => (m, None). (* TODO send error ?? *)
+
+Definition LiftOption (T : Set) (may : option T) : serverM T := fun m => (m, may).
+
+Definition Bind (T1 T2 : Set) (M1 : serverM T1) (M2 : T1 -> serverM T2) : serverM T2 :=
   fun m =>
     let (m', v1) := M1 m in
-      M2 v1 m'.
+    match v1 with
+    | Some v => M2 v m'
+    | None => (m', None)
+    end.
 
 Class Monad (M : Set -> Set) := {
-  Return {T: Set} (v: T) : M T ;
-  Bind {T1 T2 : Set} (M1 : M T1) (M2 : T1 -> M T2) : M T2
+  MReturn {T: Set} (v: T) : M T ;
+  MBind {T1 T2 : Set} (M1 : M T1) (M2 : T1 -> M T2) : M T2
  }.
 
-Instance monad_stateM : Monad stateM :=
- { Return := SReturn; Bind := SBind }.
+Instance monad_serverM : Monad serverM :=
+ { MReturn := Return; MBind := Bind }.
 
-Notation "x <- m1 ; m2" := (Bind m1 (fun x => m2))
+Notation "x <- m1 ; m2" := (MBind m1 (fun x => m2))
   (right associativity, at level 60).
-Notation "m1 ;; m2" := (Bind m1 (fun _ => m2))
+Notation "m1 ;; m2" := (MBind m1 (fun _ => m2))
   (right associativity, at level 60).
-
-Definition append (x : list ascii) (y : list ascii) : list ascii := concat [x; y].
 
 Notation "l1 <+> l2" := (append l1 l2) (right associativity, at level 30).
 (*
@@ -75,11 +87,13 @@ Instance monad_readMessageM : Monad readMessageM :=
     Bind T1 T2 M1 M2 := fun m =>
     let (m', v1) := M1 m in
       M2 v1 m' }.
-*)
+ *)
+
+(*
 Section mspec.
    Variables (T : Set) (P : state -> T -> Prop).
 
-   Definition mspec (m1 : stateM T) (m : state) : Prop :=
+   Definition mspec (m1 : serverM T) (m : state) : Prop :=
     P (fst (m1 m)) (snd (m1 m)).
 
    Lemma mspec_Return : forall m v,
@@ -93,7 +107,7 @@ Section mspec_imp.
    Variable T : Set.
    Variables P1 P2 : state -> T -> Prop.
   
-   Variable m1 : stateM T.
+   Variable m1 : serverM T.
    Variable m : state.
 
   Theorem mspec_imp : mspec P1 m1 m
@@ -103,7 +117,7 @@ Section mspec_imp.
     intuition.
   Qed.
 End mspec_imp.
-
+*)
 (*Section mspec_Read.
    Variable P : memory -> nat -> Prop.
   
@@ -121,15 +135,15 @@ End mspec_Read.
 Section mspec_Bind.
    Variables (T1 T2 : Set) (P : state -> T2 -> Prop).
 
-   Variable m1 : stateM T1.
-   Variable m2 : T1 -> stateM T2.
+   Variable m1 : serverM T1.
+   Variable m2 : T1 -> serverM T2.
 
   Theorem mspec_Bind : forall m,
     mspec (fun m v => mspec P (m2 v) m) m1 m
     -> mspec P (Bind m1 m2) m.
     unfold mspec, Bind, SBind; simpl; intro.
     destruct (m1 m); simpl.
-    destruct (m2 t m). unfold SBind. intro. unfold stateM in m1, m2. auto. 
+    destruct (m2 t m). unfold SBind. intro. unfold serverM in m1, m2. auto. 
     destruct (m1 m). destruct (m2 t1 s1). destruct (m2 t s) in H. intuition.
 
   Qed.
@@ -141,79 +155,107 @@ Definition opDATA := 3.
 Definition opACK := 4.
 Definition opERROR := 5.
 
-Definition get_2b_int (msg : message) : maybe nat := match msg with
-  | a :: b :: _ => just ( (256 * (nat_of_ascii a) + (nat_of_ascii b)))
-  | _ => nothing nat
+Inductive TFTPMessage : Set
+  := RRQ (filename : string)
+   | WRQ (filename : string)
+   | ERROR (code : N) (message : string)
+   | DATA (block : N) (data : string)
+   | ACK (block : N).
+
+Definition get_2b_int (msg : message) : option nat := match msg with
+  | String a (String b _) => Some ( (256 * (nat_of_ascii a) + (nat_of_ascii b)))
+  | _ => None
   end.
 
-Definition nat_to_2b (n : nat) : message := [(ascii_of_nat (n / 256)); (ascii_of_nat n)].
+Definition nat_to_2b (n : nat) : message := String (ascii_of_nat (n / 256)) (String (ascii_of_nat n) EmptyString).
 
-Definition get_message_id (msg : message) : maybe nat := get_2b_int msg.
+(* TODO *)
+Definition Serialize (msg : TFTPMessage) : string :=
+  match msg with
+    | RRQ filename => EmptyString
+    | WRQ filename => EmptyString
+    | ERROR code message => EmptyString
+    | DATA block data => EmptyString
+    | ACK block => EmptyString
+                    end.
 
-Fixpoint drop {T : Set} (n: nat) (l : list T) : list T := match (n, l) with
+Definition Deserialize (data : string) : option TFTPMessage :=
+  None.
+
+Theorem SerializationCorrectness : forall m : TFTPMessage, Deserialize (Serialize m) = Some m.
+  intros.
+  unfold Serialize.
+  unfold Deserialize.
+  admit.
+Admitted. (* TODO *)
+
+Definition get_message_id (msg : message) : option nat := get_2b_int msg.
+
+Fixpoint drop (n: nat) (l : string) : string := match (n, l) with
   | (O, l) => l
-  | (_, []) => []
-  | (S k, _ :: t) => drop k t
+  | (_, EmptyString) => EmptyString
+  | (S k, String _ t) => drop k t
   end.
 
-Definition get_block_id (msg : message) : maybe nat := get_2b_int (drop 2 msg).
+Definition get_block_id (msg : message) : option nat := get_2b_int (drop 2 msg).
 
-Definition make_RRQ (filename: list ascii) : message :=
-  concat [[zero; ascii_of_nat opRRQ]; filename; [zero]; ["o"; "c"; "t"; "e"; "t"]; [zero]].
 
-Definition initialize (tid : N) (port : N) (f : list ascii): state * action :=
-  (mkState waiting_for_init_ack (nothing message) tid, send (make_RRQ f) port).
 
-Definition fail : stateM action := Return terminate. (* TODO send error *)
+(* Definition make_RRQ (filename: string) : message := *)
+(*   concat [[zero; ascii_of_nat opRRQ]; filename; [zero]; ["o"; "c"; "t"; "e"; "t"]; [zero]]. *)
 
-Definition make_ACK (blockid : nat) : message :=
-  concat [nat_to_2b opACK; nat_to_2b blockid].
+Definition initialize (tid : N) (port : N) (f : string): state :=
+  (mkState waiting_for_init_ack (None) tid [send (Serialize (RRQ f)) port]).
 
-Definition make_ERROR (errid : nat) : message :=
-  concat [nat_to_2b opERROR; nat_to_2b errid; [zero]].
+(* Definition make_ACK (blockid : nat) : message := *)
+(*   concat [nat_to_2b opACK; nat_to_2b blockid]. *)
 
-Definition get_data : message -> list ascii := drop 4.
+(* Definition make_ERROR (errid : nat) : message := *)
+(*   concat [nat_to_2b opERROR; nat_to_2b errid; [zero]]. *)
 
-Definition data_length (msg : message) : nat := length (get_data msg).
+(* Definition get_data : message -> string := drop 4. *)
 
-Definition handle_incoming_data (sender : N) (blockid : nat) (msg : message) : stateM action :=
-  SetFSM (waiting_for_next_packet sender (blockid + 1));;
-  (if data_length msg <? 512 then
-    (* this was the last block, finish up *)
-    SetFSM finished
-  else
-    Return tt);;
-  Return (send (make_ACK blockid) sender).
+(* Definition data_length (msg : message) : nat := length (get_data msg). *)
 
-Definition process_step (event : input_event) : stateM action :=
+(* Definition handle_incoming_data (sender : N) (blockid : nat) (msg : message) : serverM unit := *)
+(*   (* TODO write data to file *) *)
+(*   SetFSM (waiting_for_next_packet sender (blockid + 1));; *)
+(*   (if data_length msg <? 512 then *)
+(*     (* this was the last block, finish up *) *)
+(*     SetFSM finished *)
+(*   else *)
+(*     Return tt);; *)
+(*   Send (make_ACK blockid) sender. *)
+
+Definition process_step (event : input_event) : serverM unit :=
   match event with
-  | incoming msg sender => 
+  | incoming msg sender =>
+    tftpmsg <- LiftOption (Deserialize msg);
     st <- GetFSM;
     match st with
-    | waiting_for_init_ack => match get_message_id msg with
-      | just 3 => match get_block_id msg with
-          | just 1 => handle_incoming_data sender 1 msg
-          | _ => fail
-          end
-      | _ => fail
+    | waiting_for_init_ack => match tftpmsg with
+      | DATA 1 data => Fail unit
+          (* | Some 1 => handle_incoming_data sender 1 msg *)
+      | _ => Fail unit
       end
-    | errored => Return (terminate)
-    | waiting_for_next_packet sendertid expectedblockid => 
-       if N.eqb sender sendertid then
-         match get_message_id msg with
-         | just 3 => match get_block_id msg with
-            | just incomingblockid =>
-                if incomingblockid =? expectedblockid then
-                  handle_incoming_data sender incomingblockid msg
-                else if incomingblockid <? expectedblockid then
-                  Return continue (* probably earlier block has been retransmitted, so we ignore it *)
-                else fail
-            | _ => fail
-            end
-         | _ => fail
+    | errored => Fail unit (* TODO ? *)
+    | waiting_for_next_packet sendertid expectedblockid =>
+       if N.eqb sender sendertid then (* check if we received the message from the server or somwehere else and if the source is incorrect, send an error and continue *)
+         match tftpmsg with
+           | _ => Fail unit
+         (* | Some 3 => match get_block_id msg with *)
+         (*    | Some incomingblockid => *)
+         (*        if incomingblockid =? expectedblockid then *)
+         (*          handle_incoming_data sender incomingblockid msg *)
+         (*        else if incomingblockid <? expectedblockid then *)
+         (*          Return tt (* probably earlier block has been retransmitted, so we ignore it *) *)
+         (*        else Fail unit *)
+         (*    | _ => Fail unit *)
+         (*    end *)
+         (* | _ => Fail unit *)
          end
-       else Return (send (make_ERROR 5) sender)
-    | finished => Return (terminate)
+       else Send (Serialize (ERROR 5 "Unknown transfer ID")) sender
+    | finished => Fail unit (* TODO *)
     end
-  | timeout => Return (terminate)
+  | timeout => Fail unit (* TODO *)
   end.
